lawyer/nonblocking/mk_ref.v
@@ -1,0 +1,42 @@
+From iris.proofmode Require Import tactics.
+From lawyer Require Import program_logic sub_action_em action_model.
+From lawyer.examples Require Import obls_tactics.
+From lawyer.obligations Require Import obligations_resources obligations_logic env_helpers obligations_model.
+From heap_lang Require Import lang.
+
+
+Section SimpleExample.
+
+  Definition mk_ref: val :=
+    λ: "v",
+      let: "l" := ref "v" in
+      "l"
+  .
+
+  Context {DegO LvlO LIM_STEPS} {OP: OP_HL DegO LvlO LIM_STEPS}.
+  Context `{EM: ExecutionModel heap_lang M}.
+
+  Context {Σ} {OHE: OM_HL_Env OP EM Σ}.
+
+  Notation "'Degree'" := (om_hl_Degree).
+  Context (d: Degree).
+
+  Existing Instance OHE. 
+
+  Lemma mk_ref_spec τ π q (a: val):
+    {{{ cp_mul π d 5 ∗ th_phase_frag τ π q }}}
+        mk_ref a @ τ
+    {{{ (l: loc), RET #l; l ↦ a ∗ th_phase_frag τ π q }}}.
+  Proof using.
+    iIntros (Φ) "(CPS & PH) POST". rewrite /mk_ref.
+    pure_steps.
+    wp_bind (ref _)%E.
+    iApply sswp_MU_wp; [done| ].
+    iApply wp_alloc. iModIntro. iIntros (l) "L _".
+    MU_by_burn_cp.
+    pure_steps.
+    wp_bind (Rec _ _ _)%E. pure_steps.
+    iApply "POST". by iFrame.
+  Qed.
+
+End SimpleExample.
