lawyer/nonblocking/om_wfree_inst.v
@@ -1,0 +1,34 @@
+From iris.proofmode Require Import tactics.
+(* From lawyer Require Import program_logic sub_action_em action_model. *)
+From lawyer.examples Require Import orders_lib.
+From lawyer.obligations Require Import env_helpers obligations_model .
+
+
+Definition WF_Degree := bounded_nat 2.
+Definition WF_Level := unit.
+Definition WF_SB := 1.
+
+Instance OPP_WF: ObligationsParamsPre WF_Degree WF_Level WF_SB.
+esplit; try by apply _.
+- apply nat_bounded_PO.
+- apply unit_PO.
+Defined.
+
+
+Instance OP_HL_WF: OP_HL WF_Degree WF_Level WF_SB := {| om_hl_OPRE := OPP_WF |}.
+
+
+Definition d_wfr0: WF_Degree. refine (ith_bn 2 0 _). abstract lia. Defined.
+Definition d_wfr1: WF_Degree. refine (ith_bn 2 1 _). abstract lia. Defined.
+Definition l_wfr: WF_Level := tt.
+
+
+Declare Scope WFR_scope.
+
+Notation "'d0'" := (d_wfr0) : WFR_scope.
+Notation "'d1'" := (d_wfr1) : WFR_scope.
+Notation "'l0'" := (l_wfr) : WFR_scope.
+
+Notation "'Degree'" := (WF_Degree) : WFR_scope.
+Notation "'Level'" := (WF_Level) : WFR_scope.
+
